src/Examples/ExMach/WeakestPre.v
@@ -5,42 +5,38 @@ From iris.algebra Require Export functions.
 From iris.base_logic.lib Require Export invariants gen_heap.
 From iris.proofmode Require Export tactics.
 Require Export ExMach.ExMachAPI.
-Require Export ExMach.SeqHeap.
 Set Default Proof Using "Type".
-
-Class exmachGenG Σ := ExMachGenG {
-                     exm_gen_invG : invG Σ;
-                     exm_gen_mem_inG :> seq_heapG nat nat Σ;
-                     exm_gen_disk_inG :> gen_heapG nat nat Σ;
-                   }.
 
 Class exmachG Σ := ExMachG {
                      exm_invG : invG Σ;
-                     exm_mem_inG :> seq_heapG nat nat Σ;
+                     exm_mem_inG :> gen_heapG nat nat Σ;
                      exm_disk_inG :> gen_heapG nat nat Σ;
-                     exm_current : nat;
                    }.
-
-Definition exmachGen_set `{H: exmachGenG Σ} (k: nat) :=
-  ExMachG Σ (exm_gen_invG) (exm_gen_mem_inG) (exm_gen_disk_inG)
-          k.
 
 Import ExMach.
 
-Definition ex_mach_interp {Σ} {hG: gen_heapG addr nat Σ} {hS: seq_heapG addr nat Σ} curr :=
-      (λ s, ∃ mems disks, seq_heap_ctx mems ∗
-                          gen_heap_ctx disks ∗
-                            ⌜ mems curr = mem_state s ∧
-                              disks = disk_state s ∧
-                              (∀ k, k > curr → mems k = mem_state (crash_fun s)) ∧
-                              (∀ i, is_Some (mem_state s !! i) → i < size) ∧
-                              (∀ i, is_Some (disk_state s !! i) → i < size) ⌝
+Lemma gen_heap_strong_init `{H: gen_heapPreG L V Σ} σs :
+  (|==> ∃ (H0 : gen_heapG L V Σ) (Hpf: gen_heap_inG = gen_heap_preG_inG), gen_heap_ctx σs ∗
+    own (gen_heap_name _) (◯ (to_gen_heap σs)))%I.
+Proof.
+  iMod (own_alloc (● to_gen_heap σs ⋅ ◯ to_gen_heap σs)) as (γ) "(?&?)".
+  { apply auth_valid_discrete_2; split; auto. exact: to_gen_heap_valid. }
+  iModIntro. unshelve (iExists (GenHeapG L V Σ _ _ _ γ), _); auto. iFrame.
+Qed.
+
+Definition ex_mach_interp {Σ} {hM: gen_heapG addr nat Σ} {hD: gen_heapG addr nat Σ} :=
+      (λ s, ∃ mem disk, (gen_heap_ctx mem (hG := hM)) ∗
+                        (gen_heap_ctx disk (hG := hD)) ∗
+                        ⌜ mem = mem_state s ∧
+                          disk = disk_state s ∧
+                          (∀ i, is_Some (mem_state s !! i) → i < size) ∧
+                          (∀ i, is_Some (disk_state s !! i) → i < size) ⌝
       )%I.
 
 Instance exmachG_irisG `{exmachG Σ} : irisG ExMach.Op ExMach.l Σ :=
   {
     iris_invG := exm_invG;
-    state_interp := ex_mach_interp exm_current;
+    state_interp := @ex_mach_interp _ exm_mem_inG exm_disk_inG;
   }.
 
 
@@ -51,20 +47,17 @@ Definition mem_mapsto_vs k v k' :=
   | Gt => Some 0
   end.
 
-Global Notation "l ↦{ q } v @N" :=
-  (@mapsto_fun _ _ _ _ _ (exm_mem_inG) l q (mem_mapsto_vs (exm_current) v))
-  (at level 20, q at level 50, format "l  ↦{ q } v @N") : bi_scope.
-Global Notation "l ↦ v @N " :=
-  (@mapsto_fun _ _ _ _ _ (exm_mem_inG) l 1 (mem_mapsto_vs (exm_current) v))
+Global Notation "l m↦{ q } v " := (mapsto (hG := exm_mem_inG) l q v)
+  (at level 20, q at level 50, format "l  m↦{ q } v") : bi_scope.
+Global Notation "l m↦ v " :=
+  (mapsto (hG := exm_mem_inG) l 1 v)
   (at level 20) : bi_scope.
 
-Global Notation "l ↦{ q } v @C" :=
-  (@mapsto_fun _ _ _ _ _ (exm_mem_inG) l q (mem_mapsto_vs (S exm_current) v))
-  (at level 20, q at level 50, format "l  ↦{ q } v @C") : bi_scope.
-Global Notation "l ↦ v @C" :=
-  (@mapsto_fun _ _ _ _ _ (exm_mem_inG) l 1 (mem_mapsto_vs (S exm_current) v))
+Global Notation "l d↦{ q } v " := (mapsto (hG := exm_disk_inG) l q v)
+  (at level 20, q at level 50, format "l  d↦{ q } v") : bi_scope.
+Global Notation "l d↦ v " :=
+  (mapsto (hG := exm_disk_inG) l 1 v)
   (at level 20) : bi_scope.
-
 
 Section lifting.
 Context `{exmachG Σ}.
@@ -75,72 +68,55 @@ Lemma nat_compare_gt_Gt: ∀ n m : nat, n > m → (n ?= m) = Gt.
 Proof. intros. by apply nat_compare_gt. Qed.
 
 Lemma mem_init_to_bigOp mem:
-  own (seq_heap_name (exm_mem_inG))
-      (◯ to_seq_heap (λ i : nat, match Nat.compare i exm_current with
-                                    | Lt => ε
-                                    | Eq => mem
-                                    | Gt => (fun _ => 0) <$> mem
-                                    end))
+  own (i := @gen_heap_inG _ _ _ _ _ exm_mem_inG)
+      (gen_heap_name (exm_mem_inG))
+      (◯ to_gen_heap mem)
       -∗
-  [∗ map] i↦v ∈ mem, i ↦ v @N.
+  [∗ map] i↦v ∈ mem, i m↦ v .
 Proof.
   induction mem using map_ind.
   - iIntros. rewrite //=.
   - iIntros "Hown".
     rewrite big_opM_insert //.
 
-    iAssert (own (seq_heap_name (exm_mem_inG))
-                 (◯ to_seq_heap (λ i : nat, match Nat.compare i exm_current with
-                                            | Lt => ε
-                                            | Eq => m
-                                            | Gt => (fun _ => 0) <$> m
-                                            end))
-                 ∗
-                 (i ↦ x @N))%I
+    iAssert (own (i := @gen_heap_inG _ _ _ _ _ exm_mem_inG) (gen_heap_name (exm_mem_inG))
+                 (◯ to_gen_heap m) ∗
+                 (i m↦ x))%I
                     with "[Hown]" as "[Hrest $]".
-    { rewrite /mem_mapsto_vs mapsto_fun_eq /mapsto_fun_def.
-      rewrite -own_op.
-      iApply (own_mono with "Hown").
-      rewrite -auth_frag_op. apply auth_frag_mono.
-      exists ε. rewrite right_id.
-      intros k. rewrite ofe_fun_lookup_op. rewrite /to_seq_heap.
-      destruct (Nat.compare_spec k (exm_current)).
-      * subst. rewrite to_gen_heap_insert.
-        rewrite insert_singleton_op; first by rewrite comm.
-        by apply lookup_to_gen_heap_None.
-      * by rewrite right_id.
-      * rewrite fmap_insert to_gen_heap_insert.
-        rewrite insert_singleton_op; first by rewrite comm.
-        rewrite ?lookup_fmap H0 //=.
+    {
+      rewrite mapsto_eq /mapsto_def //.
+      rewrite to_gen_heap_insert insert_singleton_op; last by apply lookup_to_gen_heap_None.
+      rewrite auth_frag_op. iDestruct "Hown" as "(?&?)". iFrame.
     }
     by iApply IHmem.
 Qed.
 
-Lemma mem_init_to_bigOp0 mem:
-  exm_current = 0 →
-  (∀ i, is_Some (mem !! i) ↔ i < size) →
-  own (seq_heap_name (exm_mem_inG))
-      (◯ to_seq_heap (λ i : nat, if nat_eq_dec i exm_current then mem else init_zero))
+Lemma disk_init_to_bigOp disk:
+  own (i := @gen_heap_inG _ _ _ _ _ exm_disk_inG)
+      (gen_heap_name (exm_disk_inG))
+      (◯ to_gen_heap disk)
       -∗
-  [∗ map] i↦v ∈ mem, i ↦ v @N.
+  [∗ map] i↦v ∈ disk, i d↦ v .
 Proof.
-  intros H0 Hsize.
-  iIntros.
-  iApply mem_init_to_bigOp.
-  iApply own_mono; last eauto.
-  apply auth_frag_mono.
-  exists ε. rewrite right_id.
-  intros k. rewrite H0. rewrite /to_seq_heap.
-  destruct (Nat.compare_spec k 0).
-  * subst. destruct nat_eq_dec; last by exfalso. done.
-  * lia.
-  * destruct nat_eq_dec; first by lia.
-    rewrite /to_gen_heap => l.
-    rewrite well_sized_mem_0_init //.
+  induction disk using map_ind.
+  - iIntros. rewrite //=.
+  - iIntros "Hown".
+    rewrite big_opM_insert //.
+
+    iAssert (own (i := @gen_heap_inG _ _ _ _ _ exm_disk_inG) (gen_heap_name (exm_disk_inG))
+                 (◯ to_gen_heap m) ∗
+                 (i d↦ x))%I
+                    with "[Hown]" as "[Hrest $]".
+    {
+      rewrite mapsto_eq /mapsto_def //.
+      rewrite to_gen_heap_insert insert_singleton_op; last by apply lookup_to_gen_heap_None.
+      rewrite auth_frag_op. iDestruct "Hown" as "(?&?)". iFrame.
+    }
+    by iApply IHdisk.
 Qed.
 
 Lemma wp_write_mem s E i v' v :
-  {{{ ▷ i ↦ v' @N }}} write_mem i v @ s; E {{{ RET tt; i ↦ v @N }}}.
+  {{{ ▷ i m↦ v' }}} write_mem i v @ s; E {{{ RET tt; i m↦ v }}}.
 Proof.
   iIntros (Φ) ">Hi HΦ". iApply wp_lift_call_step.
   iIntros (σ) "Hown".
@@ -148,30 +124,14 @@ Proof.
   iIntros (e2 σ2 Hstep) "!>".
   inversion Hstep; subst.
   iDestruct "Hown" as (mems disks) "(Hown1&Hown2&Hp)".
-  iDestruct "Hp" as %(Heq_mem&?&Hcrash_mem&Hsize&?).
-  iDestruct (seq_heap_valid with "Hown1 Hi") as %Hin_bound.
-  iMod (@seq_heap_update _ _ _ _ _ exm_mem_inG mems i
-                         (mem_mapsto_vs (exm_current) v')
-                         (mem_mapsto_vs (exm_current) v)
-          with "Hown1 Hi") as "(Hown1&Hi)".
-  { intros k. rewrite /mem_mapsto_vs.  destruct Nat.compare => //=. clear; firstorder. }
-  iModIntro.
-  iSplitR "Hi HΦ".
+  iDestruct "Hp" as %(Heq_mem&?&Hsize&?).
+  iDestruct (gen_heap_valid with "Hown1 Hi") as %Hin_bound.
+  iMod (@gen_heap_update with "Hown1 Hi") as "[Hown1 Hi]".
+  iModIntro. iSplitR "Hi HΦ".
   - iExists _, _. iFrame.
     iPureIntro. split_and!.
-    * rewrite /mem_mapsto_vs Nat.compare_refl.
-      rewrite /set_mem/set_default//=. rewrite -Heq_mem.
-      specialize (Hin_bound exm_current v').
-      rewrite Hin_bound //.
-      rewrite /mem_mapsto_vs Nat.compare_refl //=.
+    * rewrite /set_mem/set_default -Heq_mem Hin_bound //.
     * done.
-    * intros k Hgt.
-      rewrite /mem_mapsto_vs. rewrite nat_compare_gt_Gt /=; last auto.
-      rewrite /crash_fun/set_mem. rewrite /= Hcrash_mem; last auto.
-      rewrite /crash_fun/set_mem/=.
-      apply init_zero_insert_zero. apply Hsize.
-      exists v'. rewrite -Heq_mem. apply Hin_bound.
-      rewrite /mem_mapsto_vs Nat.compare_refl //=.
     * rewrite /set_mem/set_default//= => i'.
       specialize (Hsize i').
       destruct ((mem_state σ) !! i) eqn:Heq; rewrite Heq.
@@ -184,7 +144,7 @@ Proof.
 Qed.
 
 Lemma wp_read_mem s E i v :
-  {{{ ▷ i ↦ v @N }}} read_mem i @ s; E {{{ RET v; i ↦ v @N }}}.
+  {{{ ▷ i m↦ v }}} read_mem i @ s; E {{{ RET v; i m↦ v }}}.
 Proof.
   iIntros (Φ) ">Hi HΦ". iApply wp_lift_call_step.
   iIntros (σ) "Hown".
@@ -192,27 +152,12 @@ Proof.
   iIntros (e2 σ2 Hstep) "!>".
   inversion Hstep; subst.
   iDestruct "Hown" as (mems disks) "(Hown1&Hown2&Hp)".
-  iDestruct "Hp" as %(Heq_mem&?&Hcrash_mem&Hsize&?).
-  iDestruct (seq_heap_valid with "Hown1 Hi") as %Hin_bound.
+  iDestruct "Hp" as %(Heq_mem&?&Hsize&?).
+  iDestruct (gen_heap_valid with "Hown1 Hi") as %Hin_bound.
   iModIntro. iSplitR "Hi HΦ".
   - iExists _, _. iFrame; iPureIntro; split_and!; eauto.
-  - rewrite /get_mem/get_default.
-    rewrite -Heq_mem.
-    rewrite (Hin_bound _ v).
-    * by iApply "HΦ".
-    * rewrite /mem_mapsto_vs Nat.compare_refl //=.
-Qed.
-
-Lemma mem_crash i v : i ↦ v @N -∗ i ↦ 0 @C.
-Proof.
-  eapply mapsto_fun_weaken with (k := exm_current).
-  intros k. rewrite /mem_mapsto_vs. destruct nat_eq_dec; subst.
-  - rewrite nat_compare_lt_Lt; auto.
-  - destruct (Nat.compare_spec k (exm_current)).
-    * rewrite nat_compare_lt_Lt; try congruence.
-    * rewrite nat_compare_lt_Lt; try congruence; lia.
-    * destruct (Nat.compare_spec k (S exm_current)); auto.
-      lia.
+  - rewrite /get_mem/get_default -Heq_mem Hin_bound.
+    by iApply "HΦ".
 Qed.
 
 Lemma cas_non_stuck i v1 v2 σ:
@@ -225,7 +170,7 @@ Qed.
 
 Lemma wp_cas_fail s E i v1 v2 v3 :
   v1 ≠ v2 →
-  {{{ ▷ i ↦ v1 @N }}} cas i v2 v3 @ s; E {{{ RET v1; i ↦ v1 @N }}}.
+  {{{ ▷ i m↦ v1 }}} cas i v2 v3 @ s; E {{{ RET v1; i m↦ v1 }}}.
 Proof.
   iIntros (Hneq Φ) ">Hi HΦ". iApply wp_lift_call_step.
   iIntros (σ) "Hown".
@@ -233,11 +178,10 @@ Proof.
   { destruct s; auto using cas_non_stuck. }
   iIntros (e2 σ2 Hstep) "!>".
   iDestruct "Hown" as (mems disks) "(Hown1&Hown2&Hp)".
-  iDestruct "Hp" as %(Heq_mem&?&Hcrash_mem&Hsize&?).
-  iDestruct (seq_heap_valid with "Hown1 Hi") as %Hin_bound.
+  iDestruct "Hp" as %(Heq_mem&?&Hsize&?).
+  iDestruct (gen_heap_valid with "Hown1 Hi") as %Hin_bound.
   assert (Hlookup: σ.(mem_state) !! i = Some v1).
-  { rewrite -Heq_mem. apply Hin_bound.
-    rewrite /mem_mapsto_vs Nat.compare_refl //=. }
+  { rewrite -Heq_mem. apply Hin_bound. }
   inversion Hstep as (v'&σ2'&Hread&Hrest); subst.
   rewrite /get_mem/get_default/reads Hlookup in Hread.
   inversion Hread; subst.
@@ -249,7 +193,7 @@ Proof.
 Qed.
 
 Lemma wp_cas_suc s E i v1 v2 :
-  {{{ ▷ i ↦ v1 @N }}} cas i v1 v2 @ s; E {{{ RET v1; i ↦ v2 @N }}}.
+  {{{ ▷ i m↦ v1 }}} cas i v1 v2 @ s; E {{{ RET v1; i m↦ v2 }}}.
 Proof.
   iIntros (Φ) ">Hi HΦ". iApply wp_lift_call_step.
   iIntros (σ) "Hown".
@@ -257,11 +201,10 @@ Proof.
   { destruct s; auto using cas_non_stuck. }
   iIntros (v2' σ2 Hstep) "!>".
   iDestruct "Hown" as (mems disks) "(Hown1&Hown2&Hp)".
-  iDestruct "Hp" as %(Heq_mem&?&Hcrash_mem&Hsize&?).
-  iDestruct (seq_heap_valid with "Hown1 Hi") as %Hin_bound.
+  iDestruct "Hp" as %(Heq_mem&?&Hsize&?).
+  iDestruct (gen_heap_valid with "Hown1 Hi") as %Hin_bound.
   assert (Hlookup: σ.(mem_state) !! i = Some v1).
-  { rewrite -Heq_mem. apply Hin_bound.
-    rewrite /mem_mapsto_vs Nat.compare_refl //=. }
+  { rewrite -Heq_mem. apply Hin_bound. }
   inversion Hstep as (v'&σ2'&Hread&Hrest); subst.
   inversion Hread; subst.
   rewrite /get_mem/get_default/reads Hlookup in Hread Hrest.
@@ -269,28 +212,13 @@ Proof.
   destruct Hrest as ([]&?&Hputs&Hpure).
   inversion Hpure; subst.
   inversion Hputs; inversion Hpure; subst.
-  iMod (@seq_heap_update _ _ _ _ _ exm_mem_inG mems i
-                         (mem_mapsto_vs (exm_current) _)
-                         (mem_mapsto_vs (exm_current) v2)
-          with "Hown1 Hi") as "(Hown1&Hi)".
-  { intros k. rewrite /mem_mapsto_vs.  destruct Nat.compare => //=. clear; firstorder. }
+  iMod (@gen_heap_update with "Hown1 Hi") as "(Hown1&Hi)".
   iModIntro.
   iSplitR "Hi HΦ".
   - iExists _, _. iFrame.
     iPureIntro. split_and!.
-    * rewrite /mem_mapsto_vs Nat.compare_refl.
-      rewrite /set_mem/set_default//=. rewrite -Heq_mem.
-      specialize (Hin_bound exm_current v2').
-      rewrite Hin_bound //.
-      rewrite /mem_mapsto_vs Nat.compare_refl //=.
+    * rewrite /set_mem/set_default//= Hin_bound //.
     * done.
-    * intros k Hgt.
-      rewrite /mem_mapsto_vs. rewrite nat_compare_gt_Gt /=; last auto.
-      rewrite /crash_fun/set_mem. rewrite /= Hcrash_mem; last auto.
-      rewrite /crash_fun/set_mem/=.
-      apply init_zero_insert_zero. apply Hsize.
-      exists v2'. rewrite -Heq_mem. apply Hin_bound.
-      rewrite /mem_mapsto_vs Nat.compare_refl //=.
     * rewrite /set_mem/set_default//= => i'.
       specialize (Hsize i').
       destruct ((mem_state σ2') !! i) eqn:Heq; rewrite Heq.
@@ -300,6 +228,51 @@ Proof.
       ** apply Hsize.
     * eauto.
   - iApply "HΦ". eauto.
+Qed.
+
+Lemma wp_write_disk s E i v' v :
+  {{{ ▷ i d↦ v' }}} write_disk i v @ s; E {{{ RET tt; i d↦ v }}}.
+Proof.
+  iIntros (Φ) ">Hi HΦ". iApply wp_lift_call_step.
+  iIntros (σ) "Hown".
+  iModIntro. iSplit; first by destruct s.
+  iIntros (e2 σ2 Hstep) "!>".
+  inversion Hstep; subst.
+  iDestruct "Hown" as (mems disks) "(Hown1&Hown2&Hp)".
+  iDestruct "Hp" as %(Heq_mem&Heq_disk&?&Hsize).
+  iDestruct (gen_heap_valid with "Hown2 Hi") as %Hin_bound.
+  iMod (@gen_heap_update with "Hown2 Hi") as "[Hown2 Hi]".
+  iModIntro. iSplitR "Hi HΦ".
+  - iExists _, _. iFrame.
+    iPureIntro. split_and!.
+    * done.
+    * rewrite /set_disk/set_default -Heq_disk Hin_bound //.
+    * eauto.
+    * rewrite /set_disk/set_default//= => i'.
+      specialize (Hsize i').
+      destruct ((disk_state σ) !! i) eqn:Heq; rewrite Heq.
+      ** case (decide (i = i')).
+         *** intros -> ?. apply Hsize; eauto.
+         *** intros ?. rewrite lookup_insert_ne //=.
+      ** apply Hsize.
+  - iApply "HΦ". eauto.
+Qed.
+
+Lemma wp_read_disk s E i v :
+  {{{ ▷ i d↦ v }}} read_disk i @ s; E {{{ RET v; i d↦ v }}}.
+Proof.
+  iIntros (Φ) ">Hi HΦ". iApply wp_lift_call_step.
+  iIntros (σ) "Hown".
+  iModIntro. iSplit; first by destruct s.
+  iIntros (e2 σ2 Hstep) "!>".
+  inversion Hstep; subst.
+  iDestruct "Hown" as (mems disks) "(Hown1&Hown2&Hp)".
+  iDestruct "Hp" as %(Heq_mem&Heq_disk&Hsize&?).
+  iDestruct (gen_heap_valid with "Hown2 Hi") as %Hin_bound.
+  iModIntro. iSplitR "Hi HΦ".
+  - iExists _, _. iFrame; iPureIntro; split_and!; eauto.
+  - rewrite /get_disk/get_default -Heq_disk Hin_bound.
+    by iApply "HΦ".
 Qed.
 
 Lemma wp_assert s E b:
@@ -325,7 +298,7 @@ Section lock.
   Context `{!exmachG Σ, !lockG Σ}.
 
   Definition lock_inv (γ : gname) (i: addr) (P : iProp Σ) : iProp Σ :=
-    ((i ↦ 0 @N ∗ P ∗ own γ (Excl ())) ∨ (i ↦ 1 @N))%I.
+    ((i m↦ 0 ∗ P ∗ own γ (Excl ())) ∨ (i m↦ 1))%I.
 
   Definition is_lock (N: namespace) (γ: gname) (i: addr) (P: iProp Σ) : iProp Σ :=
     (inv N (lock_inv γ i P))%I.
@@ -339,7 +312,7 @@ Section lock.
   Global Instance locked_timless γ : Timeless (locked γ).
   Proof. apply _. Qed.
 
-  Lemma lock_init N i (R: iProp Σ) E : i ↦ 0 @N -∗ R ={E}=∗ ∃ γ, is_lock N γ i R.
+  Lemma lock_init N i (R: iProp Σ) E : i m↦ 0 -∗ R ={E}=∗ ∃ γ, is_lock N γ i R.
   Proof.
     iIntros "Hl HR".
     iMod (own_alloc (Excl ())) as (γ) "Hexcl"; first done.
